pseudo separation logic with assertions of type `option map`
instead of `map -> Prop`

compiler/src/compiler/Spilling.v
@@ -14,8 +14,181 @@ Require Import compiler.Simp.
 Require Import compiler.Simulation.
 Require Import compiler.SeparationLogic.
 Require Import compiler.SpillingMapGoals.
+Require Import bedrock2.MetricLogging.
 
 Open Scope Z_scope.
+
+Module map.
+  Section MAP.
+    Context {key value} {map : map.map key value}.
+
+    Definition dom(l: map): key -> Prop := fun x => exists v, map.get l x = Some v.
+
+    Inductive mut_disj: list map -> Prop :=
+    | mut_disj_nil:
+        mut_disj []
+    | mut_disj_cons: forall m l,
+        (forall m', In m' l -> map.disjoint m m') ->
+        mut_disj l ->
+        mut_disj (m :: l).
+
+    Definition map_keys{key': Type}{map': map.map key' value}(f: key -> key'): map -> map' :=
+      map.fold (fun m' k v => map.put m' (f k) v) map.empty.
+
+    Definition join: list map -> map := List.fold_right map.putmany map.empty.
+
+    Definition splits(L R: list map): Prop := join L = join R /\ mut_disj L /\ mut_disj R.
+
+    Definition geto(a: option map)(k: key): option value :=
+      match a with
+      | Some m => map.get m k
+      | None => None
+      end.
+
+    Definition domo(a: option map): key -> Prop :=
+      match a with
+      | Some m => fun k => exists v, map.get m k = Some v
+      | None => fun k => True (* TODO depending on where it's used, this should be False *)
+      end.
+
+    Definition putmanyo(a b: option map): option map :=
+      match a, b with
+      | Some a, Some b => Some (map.putmany a b)
+      | _, _ => None
+      end.
+
+    (* domains need not be disjoint, but if they overlap, the two maps have to agree on the value *)
+    Definition agreeing_putmany{value_eqb: value -> value -> bool}{value_eq_spec: EqDecider value_eqb}
+               (a b: option map): option map :=
+      match a, b with
+      | Some a, Some b => map.fold (fun o k v => match o with
+                                                 | Some m => match map.get m k with
+                                                             | Some v' => if value_eqb v v'
+                                                                          then Some m else None
+                                                             | None => Some (map.put m k v)
+                                                             end
+                                                 | None => None
+                                                 end)
+                                   (Some a)
+                                   b
+      | _, _ => None
+      end.
+
+    Definition disj_putmany(a b: option map): option map :=
+      match a, b with
+      | Some a, Some b => map.fold (fun o k v => match o with
+                                                 | Some m => match map.get m k with
+                                                             | Some _ => None
+                                                             | None => Some (map.put m k v)
+                                                             end
+                                                 | None => None
+                                                 end)
+                                   (Some a)
+                                   b
+      | _, _ => None
+      end.
+
+    Lemma disj_putmany_empty_l: forall m: option map,
+        disj_putmany (Some map.empty) m = m.
+    Admitted.
+
+    Lemma disj_putmany_empty_r: forall m: option map,
+        disj_putmany m (Some map.empty) = m.
+    Admitted.
+
+    Context {ok : map.ok map} {key_eqb: key -> key -> bool} {key_eq_dec : EqDecider key_eqb}.
+
+    Lemma mut_disj_disjoint: forall m1 m2,
+        mut_disj [m1; m2] ->
+        map.disjoint m1 m2.
+    Proof.
+      intros. inversion H. subst. eapply H2. simpl. auto.
+    Qed.
+
+    Lemma disjoint_mut_disj: forall m1 m2,
+        map.disjoint m1 m2 ->
+        mut_disj [m1; m2].
+    Proof.
+      intros. repeat constructor; simpl; intros; subst; try contradiction.
+      destruct H0; subst; try assumption. contradiction.
+    Qed.
+
+    Lemma split_splits: forall m m1 m2,
+        map.split m m1 m2 ->
+        splits [m] [m1; m2].
+    Proof.
+      unfold map.split, splits, join. simpl. intros. destruct H. subst. split.
+      - rewrite ?map.putmany_empty_r. reflexivity.
+      - repeat constructor; simpl; intros; try contradiction.
+        destruct H; subst; firstorder idtac.
+    Qed.
+
+    Lemma splits_split: forall m m1 m2,
+        splits [m] [m1; m2] ->
+        map.split m m1 m2.
+    Proof.
+      unfold map.split, splits, join. simpl. intros. destruct H as (?&?&?).
+      apply mut_disj_disjoint in H1.
+      rewrite ?map.putmany_empty_r in H.
+      auto.
+    Qed.
+
+    Axiom split_spec: forall (M A B: map),
+        map.split M A B <-> forall k,
+          (exists v, map.get M k = Some v /\
+                     ((map.get A k = Some v /\ map.get B k = None) \/
+                      (map.get B k = Some v /\ map.get A k = None))) \/
+          (map.get M k = None /\ map.get A k = None /\ map.get B k = None).
+
+    Axiom putmany_spec: forall (m1 m2: map) k,
+        (exists v, map.get (map.putmany m1 m2) k = Some v /\
+                   (map.get m2 k = Some v \/ (map.get m2 k = None /\ map.get m1 k = Some v))) \/
+        (map.get (map.putmany m1 m2) k = None /\ map.get m2 k = None /\ map.get m1 k = None).
+
+    Axiom getmany_of_list_shrink: forall (l l1 l2: map) keys,
+        map.split l l1 l2 ->
+        Forall (fun k => map.get l2 k = None) keys ->
+        map.getmany_of_list l keys = map.getmany_of_list l1 keys.
+
+    Axiom putmany_of_list_zip_split: forall (l l' l1 l2: map) keys values,
+        map.putmany_of_list_zip keys values l = Some l' ->
+        map.split l l1 l2 ->
+        Forall (fun k => map.get l2 k = None) keys ->
+        exists l1', map.split l' l1' l2 /\ map.putmany_of_list_zip keys values l1 = Some l1'.
+
+    Axiom putmany_of_list_zip_grow: forall (l l1 l1' l2: map) keys values,
+        map.putmany_of_list_zip keys values l1 = Some l1' ->
+        map.split l l1 l2 ->
+        Forall (fun k => map.get l2 k = None) keys ->
+        exists l', map.split l' l1' l2 /\ map.putmany_of_list_zip keys values l = Some l'.
+
+    Lemma getmany_of_list_preserved: forall (l1 l2: map) ks,
+        (forall k, In k ks -> map.get l1 k = map.get l2 k) ->
+        map.getmany_of_list l1 ks = map.getmany_of_list l2 ks.
+    Proof.
+      induction ks; intros. 1: reflexivity.
+      unfold map.getmany_of_list in *. simpl.
+      rewrite IHks. 2: {
+        intros. eapply H. simpl. auto.
+      }
+      specialize (H a). simpl in H. rewrite H. 2: auto.
+      reflexivity.
+    Qed.
+
+    (* disjoint-unions *)
+    Definition dus'(l: list (option map)): option map :=
+      List.fold_left (fun res e => disj_putmany res e) l (Some map.empty).
+
+    Fixpoint dus (xs : list (option map)) : option map :=
+      match xs with
+      | [x] => x
+      | x :: xs => disj_putmany (dus xs) x
+      | nil => Some map.empty
+      end.
+
+  End MAP.
+End map.
+
 
 Section Spilling.
 
@@ -39,7 +212,7 @@ Section Spilling.
 
   (* Definition needs_spilling: Z -> bool := Z.leb 32. *)
 
-  Context {W: Utility.Words} {mem: map.map word byte}.
+  Context {W: Utility.Words} {mem: map.map word byte} {mem_ok: map.ok mem}.
 
   Definition stack_loc(r: Z): option Z :=
     if Z.leb 32 r then Some ((r - 32) * bytes_per_word) else None.
@@ -179,7 +352,7 @@ Section Spilling.
   Proof.
     (* Wihtout the clear, firstorder becomes very slow COQBUG https://github.com/coq/coq/issues/11352.
        Not using firstorder though because there's something higher order here: *)
-    clear mem locals localsOk env ext_spec.
+    clear mem mem_ok locals localsOk env ext_spec.
     assert (forall vars, Forall (fun x : Z => 5 < x < 32) vars -> Forall (fun x : Z => 2 < x < 32) vars). {
       intros. eapply Forall_impl. 2: eassumption. simpl. blia.
     }
@@ -206,172 +379,107 @@ Section Spilling.
       intuition try blia.
   Qed.
 
-  Definition related_old(maxvar: Z)(frame: mem)(done: bool):
-    FlatImp.SimState Z -> FlatImp.SimState Z -> Prop :=
-    fun '(t1, m1, l1, mc1) '(t2, m2, l2, mc2) =>
-      exists fpval mL mStack,
+  Definition oeq{T: Type}(oL oR: option T): Prop := exists L R, oL = Some L /\ oR = Some R /\ oL = oR.
+
+  Notation "a \+/ b" := (map.disj_putmany a b) (at level 34, left associativity).
+  Notation "a \</ b" := (map.putmanyo a b) (at level 34, left associativity).
+  Notation "a \?/ b" := (map.agreeing_putmany a b) (at level 34, left associativity).
+  Notation "k ~> v" := (Some (map.put map.empty k v)) (at level 30).
+
+  Infix "==" := oeq (at level 38).
+
+  Definition one(sz: Syntax.access_size.access_size)(addr value: word): option mem :=
+    Some (map.putmany_of_tuple (Memory.footprint addr (@Memory.bytes_per width sz))
+                               (LittleEndian.split (@Memory.bytes_per width sz) (word.unsigned value))
+                               map.empty).
+
+  Definition array{T: Type}(elem: word -> T -> option mem)(size: word): word -> list T -> option mem :=
+    fix rec addr ls :=
+      match ls with
+      | [] => Some map.empty
+      | e :: es => elem addr e \+/ rec (word.add addr size) es
+      end.
+
+  Definition word_array: word -> list word -> option mem :=
+    array (one Syntax.access_size.word) (word.of_Z bytes_per_word).
+
+  Definition related(maxvar: Z)(frame: option mem)(done: bool)
+             (t1: trace)(m1: option mem)(l1: option locals)(mc1: MetricLog)
+             (t2: trace)(m2: option mem)(l2: option locals)(mc2: MetricLog): Prop :=
+      exists fpval tmp1val tmp2val lStack lRegs stackwords,
         t1 = t2 /\
-        map.split m2 m1 mL /\ map.split mL mStack frame /\
-        (forall r, r < fp -> map.get l1 r = None) /\
-        map.get l2 fp = Some fpval /\
-        (forall r, fp < r < 32 -> map.get l1 r = map.get l2 r) /\
-        (forall r, 32 <= r < maxvar -> exists v,
-              Memory.load Syntax.access_size.word mStack
-                          (word.add fpval (word.of_Z ((r - 32) * bytes_per_word))) = Some v /\
-              forall v', map.get l1 r = Some v' -> v' = v).
+        m2 == m1 \+/ word_array fpval stackwords \+/ frame /\
+        subset (map.domo lRegs) (fun x => fp < x < 32) /\
+        subset (map.domo lStack) (fun x => 32 <= x <= maxvar) /\
+        l1 = lRegs \+/ lStack /\
+        l2 = lRegs \+/ tmp1 ~> tmp1val \+/ tmp2 ~> tmp2val \+/ fp ~> fpval /\
+        forall r, 32 <= r <= maxvar -> forall v, map.geto lStack r = Some v ->
+           nth_error stackwords (Z.to_nat (r - 32)) = Some v.
 
-  (* could be treated as a separation logic assertion *)
-  Definition spilled_vars(fpval: word)(maxvar: Z)(lStack: locals)(mStack: mem): Prop :=
-    forall r, 32 <= r <= maxvar -> exists v,
-        Memory.load Syntax.access_size.word mStack
-                    (word.add fpval (word.of_Z ((r - 32) * bytes_per_word))) = Some v /\
-        forall v', map.get lStack r = Some v' -> v' = v.
-
-  Definition split_at(l: locals)(l1: locals)(b: Z)(l2: locals): Prop :=
-    map.split l l1 l2 /\
-    (forall r v, map.get l1 r = Some v -> r < b) /\
-    (forall r v, map.get l2 r = Some v -> b <= r).
-
-  Definition related_old1(maxvar: Z)(frame: mem)(done: bool):
-    FlatImp.SimState Z -> FlatImp.SimState Z -> Prop :=
-    fun '(t1, m1, l1, mc1) '(t2, m2, l2, mc2) =>
-      exists fpval tmp1val tmp2val mL mStack lStack lRegs,
-        t1 = t2 /\
-        map.split m2 m1 mL /\ map.split mL mStack frame /\
-        split_at l1 lRegs 32 lStack /\
-        split_at l2 (map.of_list [(tmp1, tmp1val); (tmp2, tmp2val); (fp, fpval)]) regvar0 lRegs.
-
-  Definition map__dom_in(l: locals)(P: Z -> Prop): Prop := forall v r, map.get l r = Some v -> P r.
-
-  Definition map__dom(l: locals): Z -> Prop := fun x => exists v, map.get l x = Some v.
-
-  Axiom map__dom_in_put: forall (l: locals) k v P,
-      map__dom_in l P ->
-      P k ->
-      map__dom_in (map.put l k v) P.
-
-  Lemma map__split_dom_in: forall (l l1 l2: locals) P1 P2,
-      map.split l l1 l2 ->
-      map__dom_in l1 P1 ->
-      map__dom_in l2 P2 ->
-      map__dom_in l (fun x => P1 x \/ P2 x).
-  Proof.
-    unfold map.split, map__dom_in, map.disjoint. intros. simp.
-    rewrite map.get_putmany_dec in H2.
-    destr (map.get l2 r); simp; intuition eauto.
-  Qed.
-
-  Lemma map__putmany_of_list_zip_dom_in: forall (l l': locals) ks vs P,
-      map.putmany_of_list_zip ks vs l = Some l' ->
-      map__dom_in l P ->
-      map__dom_in l' (fun x => P x \/ List.In x ks).
-  Admitted.
-
-  Lemma map__split_dom_disjoint: forall l l1 l2,
-      map.split l l1 l2 ->
-      disjoint (map__dom l1) (map__dom l2).
-  Proof.
-    clear.
-    unfold map.split, map.disjoint, map__dom, disjoint, elem_of. intros *. intros [_ ?] ?.
-    specialize (H x).
-    destruct (map.get l1 x); destruct (map.get l2 x); try firstorder congruence.
-    exfalso. eauto.
-  Qed.
-
-  Lemma map__split_dom_spec: forall l l1 l2,
-      map.split l l1 l2 ->
-      disjoint (map__dom l1) (map__dom l2) /\
-      sameset (union (map__dom l1) (map__dom l2)) (map__dom l).
-  Proof.
-    clear -localsOk. split. 1: eauto using map__split_dom_disjoint.
-    unfold map.split, union, map__dom, sameset, subset, elem_of in *.
-    destruct H. subst. split; intros.
-    - rewrite map.get_putmany_dec. destruct H as [[? ?] | [? ?]]; rewrite H.
-      2: eauto. destruct (map.get l2 x); eauto.
-    - rewrite map.get_putmany_dec in H. destruct H as [? ?].
-      clear localsOk. destruct (map.get l2 x); firstorder congruence.
-  Qed.
-
-  Lemma map__split_dom_spec': forall l l1 l2,
-      map.split l l1 l2 ->
-      disjoint (map__dom l1) (map__dom l2) /\
-      union (map__dom l1) (map__dom l2) = map__dom l.
-  Proof.
-    clear -localsOk. split. 1: eauto using map__split_dom_disjoint.
-    unfold map.split, union, map__dom, elem_of in *.
-    apply iff1ToEq. destruct H. subst. split; intros.
-    - rewrite map.get_putmany_dec. destruct H as [[? ?] | [? ?]]; rewrite H.
-      2: eauto. destruct (map.get l2 x); eauto.
-    - rewrite map.get_putmany_dec in H. destruct H as [? ?].
-      clear localsOk. destruct (map.get l2 x); firstorder congruence.
-  Qed.
-
-(*
-  Lemma map__dom_in_split_l: forall (l l1 l2: locals) P,
-      map.split l l1 l2 ->
-      map__dom_in l2 P ->
-      map__dom_in l1 (fun x => ~ P x).
-  Proof.
-*)
+  (*
+  Notation "m [ k := v ]" := (map.put m k v) (at level 10, left associativity, format "m [ k  :=  v ]").
+  Notation "m [ k ]" := (map.get m k) (at level 10, left associativity, format "m [ k ]").
+  (* this notation overrides the notation for applying a function m to the singleton list containing k,
+     but that's so rare that it's fine *)
 
   Definition related(maxvar: Z)(frame: mem)(done: bool):
     FlatImp.SimState Z -> FlatImp.SimState Z -> Prop :=
     fun '(t1, m1, l1, mc1) '(t2, m2, l2, mc2) =>
-      exists fpval tmp1val tmp2val mL mStack lStack lRegs,
+      exists fpval tmp1val tmp2val mStack lStack lRegs,
         t1 = t2 /\
-        map.split m2 m1 mL /\ map.split mL mStack frame /\
-        map__dom_in lRegs (fun x => fp < x < 32) /\
-        map__dom_in lStack (fun x => 32 <= x <= maxvar) /\
-        map.split l1 lRegs lStack /\
-        map.split l2 lRegs (map.of_list [(tmp1, tmp1val); (tmp2, tmp2val); (fp, fpval)]) /\
+        m2 = map.putmany m1 (map.putmany mStack frame) /\
+        disjoint (map.dom m1) (map.dom mStack) /\
+        disjoint (map.dom m1) (map.dom frame) /\
+        disjoint (map.dom mStack) (map.dom frame) /\
+        subset (map.dom lRegs) (fun x => fp < x < 32) /\
+        subset (map.dom lStack) (fun x => 32 <= x <= maxvar) /\
+        l1 = map.putmany lRegs lStack /\
+        l2 = lRegs[tmp1 := tmp1val][tmp2 := tmp2val][fp := fpval] /\
         spilled_vars fpval maxvar lStack mStack.
+
+  Definition related(maxvar: Z)(frame: option mem)(done: bool)
+             (t1: trace)(m1: option mem)(l1: option locals)(mc1: MetricLog)
+             (t2: trace)(m2: option mem)(l2: option locals)(mc2: MetricLog): Prop :=
+      exists fpval tmp1val tmp2val mStack lStack lRegs,
+        t1 = t2 /\
+        m2 = m1 \+/ mStack \+/ frame /\
+        subset (map.domo lRegs) (fun x => fp < x < 32) /\
+        subset (map.domo lStack) (fun x => 32 <= x <= maxvar) /\
+        l1 = lRegs \+/ lStack /\
+        l2 = lRegs \+/ tmp1 ~> tmp1val \+/ tmp2 ~> tmp2val \+/ fp ~> fpval /\
+        spilled_vars fpval maxvar lStack mStack.
+
+  Definition related(maxvar: Z)(frame: mem)(done: bool):
+    FlatImp.SimState Z -> FlatImp.SimState Z -> Prop :=
+    fun '(t1, m1, l1, mc1) '(t2, m2, l2, mc2) =>
+      exists fpval tmp1val tmp2val mStack lStack lRegs,
+        t1 = t2 /\
+        Some m2 = Some m1 \+/ Some mStack \+/ Some frame /\
+        subset (map.dom lRegs) (fun x => fp < x < 32) /\
+        subset (map.dom lStack) (fun x => 32 <= x <= maxvar) /\
+        Some l1 = Some lRegs \+/ Some lStack /\
+        Some l2 = Some lRegs \+/ tmp1 ~> tmp1val \+/ tmp2 ~> tmp2val \+/ fp ~> fpval /\
+        spilled_vars fpval maxvar lStack mStack.
+
+  Notation "k ~> v" := (map.put map.empty k v) (at level 30).
+
+  Definition related(maxvar: Z)(frame: mem)(done: bool):
+    FlatImp.SimState Z -> FlatImp.SimState Z -> Prop :=
+    fun '(t1, m1, l1, mc1) '(t2, m2, l2, mc2) =>
+      exists fpval tmp1val tmp2val mStack lStack lRegs,
+        t1 = t2 /\
+        map.splits [m2] [m1; mStack; frame] /\
+        subset (map.dom lRegs) (fun x => fp < x < 32) /\
+        subset (map.dom lStack) (fun x => 32 <= x <= maxvar) /\
+        map.splits [l1] [lRegs; lStack] /\
+        map.splits [l2] [lRegs; tmp1 ~> tmp1val; tmp2 ~> tmp2val; fp ~> fpval] /\
+        spilled_vars fpval maxvar lStack mStack.
+*)
 
   Definition envs_related(e1 e2: env): Prop :=
     forall f argvars resvars body1,
       map.get e1 f = Some (argvars, resvars, body1) ->
       map.get e2 f = Some (argvars, resvars, spill_fbody body1).
-
-  Axiom map__split_spec: forall (M A B: mem),
-      map.split M A B <-> forall k,
-        (exists v, map.get M k = Some v /\
-                   ((map.get A k = Some v /\ map.get B k = None) \/
-                    (map.get B k = Some v /\ map.get A k = None))) \/
-        (map.get M k = None /\ map.get A k = None /\ map.get B k = None).
-
-  Axiom map__putmany_spec: forall (m1 m2: mem) k,
-      (exists v, map.get (map.putmany m1 m2) k = Some v /\
-                 (map.get m2 k = Some v \/ (map.get m2 k = None /\ map.get m1 k = Some v))) \/
-      (map.get (map.putmany m1 m2) k = None /\ map.get m2 k = None /\ map.get m1 k = None).
-
-  Axiom map__getmany_of_list_shrink: forall (l l1 l2: locals) keys,
-      map.split l l1 l2 ->
-      Forall (fun k => map.get l2 k = None) keys ->
-      map.getmany_of_list l keys = map.getmany_of_list l1 keys.
-
-  Axiom map__putmany_of_list_zip_split: forall (l l' l1 l2: locals) keys values,
-      map.putmany_of_list_zip keys values l = Some l' ->
-      map.split l l1 l2 ->
-      Forall (fun k => map.get l2 k = None) keys ->
-      exists l1', map.split l' l1' l2 /\ map.putmany_of_list_zip keys values l1 = Some l1'.
-
-  Axiom map__putmany_of_list_zip_grow: forall (l l1 l1' l2: locals) keys values,
-      map.putmany_of_list_zip keys values l1 = Some l1' ->
-      map.split l l1 l2 ->
-      Forall (fun k => map.get l2 k = None) keys ->
-      exists l', map.split l' l1' l2 /\ map.putmany_of_list_zip keys values l = Some l'.
-
-  Lemma map__getmany_of_list_preserved: forall (l1 l2: locals) ks,
-      (forall k, In k ks -> map.get l1 k = map.get l2 k) ->
-      map.getmany_of_list l1 ks = map.getmany_of_list l2 ks.
-  Proof.
-    induction ks; intros. 1: reflexivity.
-    unfold map.getmany_of_list in *. simpl.
-    rewrite IHks. 2: {
-      intros. eapply H. simpl. auto.
-    }
-    specialize (H a). simpl in H. rewrite H. 2: auto.
-    reflexivity.
-  Qed.
 
   Lemma seq_cps: forall e s1 s2 t m l mc post,
       exec e s1 t m l mc (fun t' m' l' mc' => exec e s2 t' m' l' mc' post) ->
@@ -379,6 +487,13 @@ Section Spilling.
   Proof.
     intros. eapply exec.seq. 1: eassumption. simpl. clear. auto.
   Qed.
+
+  Lemma load_putmany_l: forall m1 m2 sz a v,
+      Memory.load sz m1 a = Some v ->
+      disjoint (map.dom m1) (map.dom m2) ->
+      Memory.load sz (map.putmany m1 m2) a = Some v.
+  Proof.
+  Admitted.
 
   (* cps style
   Lemma load_arg_reg1_correct: forall e a t m l mc post,
@@ -390,6 +505,244 @@ Section Spilling.
       exec e s t
       exec e (SSeq (load_arg_reg1 a) s) t m l mc post. *)
 
+  Arguments map.disj_putmany : simpl never.
+
+  Implicit Types post : trace -> option mem -> option locals -> MetricLog -> Prop.
+
+  Section WithE.
+    Variable (e: env).
+
+(*
+    Definition ext_spec' t mGive action argvals (outcome: mem -> list word -> Prop) :=
+      match mGive with
+      | Some mGive => ext_spec t mGive action argvals outcome
+      | None => False
+      end.
+
+    Definition ext_spec' t mGive action argvals (outcome: option mem -> list word -> Prop) :=
+      match mGive with
+      | Some mGive => ext_spec t mGive action argvals
+                               (fun mReceive resvals => outcome (Some mReceive) resvals)
+      | None => False
+      end.
+*)
+
+    Inductive exec:
+      stmt ->
+      trace -> option mem -> option locals -> MetricLog ->
+      (trace -> option mem -> option locals -> MetricLog -> Prop)
+    -> Prop :=
+    | interact: forall t m mKeep mGive l l_not_read l_not_written oldresvals mc action argvars
+                       argvals resvars outcome post,
+        m == mKeep \+/ Some mGive ->
+        l == l_not_read \+/ map.of_list_zip argvars argvals ->
+        l == l_not_written \+/ map.of_list_zip resvars oldresvals ->
+        ext_spec t mGive action argvals outcome ->
+        (forall mReceive resvals,
+            outcome mReceive resvals ->
+            exists l', l' == l_not_written \+/ map.of_list_zip resvars resvals /\
+            forall m', m' == mKeep \+/ Some mReceive ->
+            post (((mGive, action, argvals), (mReceive, resvals)) :: t) m' l'
+                 (addMetricInstructions 1
+                 (addMetricStores 1
+                 (addMetricLoads 2 mc)))) ->
+        exec (SInteract resvars action argvars) t m l mc post
+
+    | call: forall t m l mc binds fname args params rets fbody (*argvs st0*) post (* outcome *),
+        map.get e fname = Some (params, rets, fbody) ->
+        (* TODO
+        map.getmany_of_list l args = Some argvs ->
+        map.putmany_of_list_zip params argvs map.empty = Some st0 ->
+        exec fbody t m st0 mc outcome ->
+        (forall t' m' mc' st1,
+            outcome t' m' st1 mc' ->
+            exists retvs l',
+              map.getmany_of_list st1 rets = Some retvs /\
+              map.putmany_of_list_zip binds retvs l = Some l' /\
+              post t' m' l' mc') ->
+              *)
+        exec (SCall binds fname args) t m l mc post
+    | load: forall t m mFrame l l' lFrame mc sz x a o v addr post,
+        l == lFrame \+/ a ~> addr ->
+        m == mFrame \+/ one sz (word.add addr (word.of_Z o)) v ->
+        l' == l \</ x ~> v ->
+        post t m l'
+             (addMetricLoads 2
+             (addMetricInstructions 1 mc)) ->
+        exec (SLoad sz x a o) t m l mc post
+    | store: forall t (m mFrame m': option mem) mc l lFrame sz a o addr v (val oldval: word) post,
+        l == lFrame \+/ (a ~> addr \?/ v ~> val) ->
+        m == mFrame \+/ one sz (word.add addr (word.of_Z o)) oldval ->
+        m' == mFrame \+/ one sz (word.add addr (word.of_Z o)) val ->
+        post t m' l
+             (addMetricLoads 1
+             (addMetricInstructions 1
+             (addMetricStores 1 mc))) ->
+        exec (SStore sz a v o) t m l mc post
+    | stackalloc: forall t mSmall l mc x n body post,
+        n mod bytes_per_word = 0 ->
+        (forall l0 a stacktrash mCombined,
+            mCombined == mSmall \+/ map.of_disjoint_list_zip (Memory.ftprint a n) stacktrash ->
+            l0 == l \</ x ~> a ->
+            exec body t mCombined l0 (addMetricLoads 1 (addMetricInstructions 1 mc))
+             (fun t' mCombined' l' mc' =>
+              exists mSmall' stacktrash',
+                mCombined' == mSmall' \+/ map.of_disjoint_list_zip (Memory.ftprint a n) stacktrash' /\
+                post t' mSmall' l' mc')) ->
+        exec (SStackalloc x n body) t mSmall l mc post
+
+(*
+    | lit: forall t m l mc x v post,
+        post t m (map.put l x (word.of_Z v))
+             (addMetricLoads 8
+             (addMetricInstructions 8 mc)) ->
+        exec (SLit x v) t m l mc post
+*)
+
+    | op: forall t m l l' lFrame mc x op y y' z z' post,
+        l == lFrame \+/ (y ~> y' \?/ z ~> z') ->
+        l' == l \</ x ~> Semantics.interp_binop op y' z' ->
+        post t m l'
+             (addMetricLoads 2
+             (addMetricInstructions 2 mc)) ->
+        exec (SOp x op y z) t m l mc post
+
+(*
+    | set: forall t m l mc x y y' post,
+        map.get l y = Some y' ->
+        post t m (map.put l x y')
+             (addMetricLoads 1
+             (addMetricInstructions 1 mc)) ->
+        exec (SSet x y) t m l mc post
+    | if_true: forall t m l mc cond  bThen bElse post,
+        eval_bcond l cond = Some true ->
+        exec bThen t m l
+             (addMetricLoads 2
+             (addMetricInstructions 2
+             (addMetricJumps 1 mc))) post ->
+        exec (SIf cond bThen bElse) t m l mc post
+    | if_false: forall t m l mc cond bThen bElse post,
+        eval_bcond l cond = Some false ->
+        exec bElse t m l
+             (addMetricLoads 2
+             (addMetricInstructions 2
+             (addMetricJumps 1 mc))) post ->
+        exec (SIf cond bThen bElse) t m l mc post
+    | loop: forall t m l mc cond body1 body2 mid1 mid2 post,
+        (* This case is carefully crafted in such a way that recursive uses of exec
+         only appear under forall and ->, but not under exists, /\, \/, to make sure the
+         auto-generated induction principle contains an IH for all recursive uses. *)
+        exec body1 t m l mc mid1 ->
+        (forall t' m' l' mc',
+            mid1 t' m' l' mc' ->
+            eval_bcond l' cond <> None) ->
+        (forall t' m' l' mc',
+            mid1 t' m' l' mc' ->
+            eval_bcond l' cond = Some false ->
+            post t' m' l'
+                 (addMetricLoads 1
+                 (addMetricInstructions 1
+                 (addMetricJumps 1 mc')))) ->
+        (forall t' m' l' mc',
+            mid1 t' m' l' mc' ->
+            eval_bcond l' cond = Some true ->
+            exec body2 t' m' l' mc' mid2) ->
+        (forall t'' m'' l'' mc'',
+            mid2 t'' m'' l'' mc'' ->
+            exec (SLoop body1 cond body2) t'' m'' l''
+                 (addMetricLoads 2
+                 (addMetricInstructions 2
+                 (addMetricJumps 1 mc''))) post) ->
+        exec (SLoop body1 cond body2) t m l mc post
+    | seq: forall t m l mc s1 s2 mid post,
+        exec s1 t m l mc mid ->
+        (forall t' m' l' mc', mid t' m' l' mc' -> exec s2 t' m' l' mc' post) ->
+        exec (SSeq s1 s2) t m l mc post
+    | skip: forall t m l mc post,
+        post t m l mc ->
+        exec SSkip t m l mc post
+*)
+.
+
+  End WithE.
+
+  Lemma mem_eq_trans: forall m1 m2 m3: option mem,
+      m1 == m2 -> m2 == m3 -> m1 == m3.
+  Admitted.
+
+  Lemma mem_eq_rewrite: forall F A L R: option mem,
+      L == R ->
+      A == L \+/ F ->
+      A == R \+/ F.
+  Admitted.
+
+  (* Note: does not hold if m is None! *)
+  Lemma mem_eq_refl: forall m A B: option mem,
+      A == B \+/ m -> (* <-- to assert that m is not None *)
+      m == m.
+  Proof.
+    unfold oeq, map.disj_putmany. intros. simp. clear. eauto.
+  Qed.
+
+  Section cancel_lemmas.
+    Let nth n xs := hd (@None mem) (skipn n xs).
+    Let remove_nth n (xs : list (option mem)) :=
+      (firstn n xs ++ tl (skipn n xs)).
+
+    Lemma mem_eq_cancel_at: forall (i j: nat) (xs ys: list (option mem)),
+        nth i xs = nth j ys ->
+        map.dus (remove_nth i xs) == map.dus (remove_nth j ys) ->
+        map.dus xs == map.dus ys.
+    Proof.
+    Admitted.
+  End cancel_lemmas.
+
+  Ltac cancel_at_indices i j :=
+    lazymatch goal with
+    | |- map.dus ?LHS == map.dus ?RHS =>
+      simple refine (mem_eq_cancel_at i j LHS RHS _ _);
+      cbn [firstn skipn List.app hd tl]
+    end.
+
+  Lemma spilling_correct (e e1 e2 : env) (Ev : envs_related e1 e2)
+        (s1 : stmt)
+  (t1 : trace)
+  (m1 : option mem)
+  (l1 : option locals)
+  (mc1 : MetricLog)
+  (post : trace -> option mem -> option locals -> MetricLog -> Prop):
+  exec e1 s1 t1 m1 l1 mc1 post ->
+  forall (frame : option mem) (maxvar : Z),
+  valid_vars_src maxvar s1 ->
+  forall (t2 : trace) (m2 : option mem) (l2 : option locals) (mc2 : MetricLog),
+  related maxvar frame false t1 m1 l1 mc1 t2 m2 l2 mc2 ->
+  exec e2 (spill_stmt s1) t2 m2 l2 mc2
+    (fun (t2' : trace) (m2' : option mem) (l2' : option locals) (mc2' : MetricLog) =>
+       exists t1' m1' l1' mc1',
+         related maxvar frame false t1' m1' l1' mc1' t2' m2' l2' mc2' /\
+         post t1' m1' l1' mc1').
+  Proof.
+    unfold related. induction 1; intros; simp; subst.
+    - (* exec.interact *)
+      eapply interact.
+      + eapply mem_eq_trans. 1: eassumption.
+        eapply mem_eq_trans.
+        * eapply mem_eq_rewrite. 1: exact H.
+          match goal with
+          | |- ?L1 \+/ ?L2 \+/ ?L3 == ?R1 \+/ ?R2 =>
+            change (map.dus [L3; L2; L1] == map.dus [R2; R1])
+          end.
+          cancel_at_indices 2%nat 1%nat. 1: reflexivity.
+          cbv [map.dus].
+          eapply mem_eq_refl.
+          eapply mem_eq_trans. 1: exact H5rl.
+          match goal with
+          | |- ?L1 \+/ ?L2 \+/ ?L3 == ?R1 \+/ ?R2 =>
+            change (map.dus [L3; L2; L1] == map.dus [R2; R1])
+          end.
+
+
+(*
   Lemma spilling_sim(e1 e2: env):
       envs_related e1 e2 ->
       forall frame s1 maxvar,
@@ -402,13 +755,53 @@ Section Spilling.
     revert frame maxvar V t2 m2 l2 mc2 R.
     unfold compile_inv, related.
     match type of Exec with
-    | exec _ _ _ _ _ _ ?P => remember P as post
+    | FlatImp.exec _ _ _ _ _ _ ?P => remember P as post
     end.
     revert post1 Heqpost.
     induction Exec; simpl; intros; simp; subst.
     - (* exec.interact *)
-      eapply @exec.interact with (mGive := mGive) (mKeep := map.putmany mKeep mL).
-      + eapply split_interact; eassumption.
+
+
+    - (* exec.interact *)
+      eapply map.split_splits in H.
+      eapply @exec.interact with (mGive := mGive) (mKeep := map.putmany mKeep (map.putmany mStack frame)).
+      + eapply map.splits_split.
+
+(*
+
+disjoint union on "option map" ?
+m \+/ mStack \+/ frame
+
+lRegs \+/ tmp1 ~> tmp1val \+/ tmp2 ~> tmp2val
+
+but what to pass to exec.interact? -> also "option map"
+
+disjoint_putmany
+
+just congruence:
+a = c ->
+b = d ->
+a \+/ b = c \+/ d
+
+*)
+      + unfold map.split in *; simp. split.
+        * remember (map.putmany mStack frame) as A.
+          rewrite <- map.putmany_assoc.
+          { erewrite <- (@map.putmany_assoc _ _ _ _ _ word.eqb_spec).
+            { f_equal.
+              apply map.putmany_comm.
+              subst A.
+
+          1: exact mem_ok.
+
+          { assert (map.ok FlatImp.mem = map.ok mem). {
+              clear.
+              reflexivity.
+
+rewrite <- (@map.putmany_assoc _ _ _ mem_ok word.eqb).
+
+
+subst. eapply split_interact; try eassumption.
       + erewrite map__getmany_of_list_shrink. 2: eassumption. 2: {
           eapply Forall_impl. 2: eassumption.
           clear -localsOk. unfold fp, tmp1, tmp2. intros.
@@ -504,7 +897,10 @@ Section Spilling.
         assert (32 <= a <= maxvar) as B by blia. specialize A with (1 := B); clear B. simp.
         eapply exec.load with (addr0 := fpval) (v1 := v0).
         * admit. (* ok *)
-        * admit. (* growing from mStack to m2 preserves Memory.load *)
+        * eapply grow_load. 1: eassumption.
+
+jj
+admit. (* growing from mStack to m2 preserves Memory.load *)
         * eapply seq_cps. eapply exec.load. {
             rewrite map.get_put_same. reflexivity.
           } {
@@ -613,16 +1009,48 @@ Section Spilling.
           5: eassumption.
           all: try eassumption.
       + admit. (* same but without spilling *)
-(*
     - (* exec.lit *)
+      admit.
     - (* exec.op *)
+      admit.
     - (* exec.set *)
+      admit.
     - (* exec.if_true *)
+      unfold prepare_bcond. destruct cond.
+      + simpl. eapply seq_cps. eapply seq_cps. simpl in *. simp.
+        unfold load_arg_reg1, arg_reg1, load_arg_reg2, arg_reg2, save_res_reg, res_reg, stack_loc.
+        destr (Z.leb 32 x).
+        * match goal with
+          | H: spilled_vars _ _ _ _ |- _ => pose proof H as A
+          end.
+          unfold spilled_vars in A.
+          assert (32 <= x <= maxvar) as B by blia.
+          specialize A with (1 := B); clear B. simp.
+          eapply exec.load with (addr := fpval).
+          { admit. }
+          {
+
+
+            Search Memory.load map.split.
+
+exact Al. eassumption. }
+
+            match goal with
+          | H: spilled_vars _ _ _ _ |- _ => pose proof H as A
+          end.
+          unfold spilled_vars in A.
+          assert (32 <= a <= maxvar) as B by blia. specialize A with (1 := B); clear B. simp.
+          eapply exec.load with (addr0 := fpval) (v1 := v0).
+        * admit. (* ok *)
+
+
     - (* exec.if_false *)
     - (* exec.loop *)
     - (* exec.seq *)
     - (* exec.skip *)
 *)
+
+
   Abort.
 
 End Spilling.
